examples/layeredeffects/LatticeAlg.fst
@@ -1,0 +1,269 @@
+module LatticeAlg
+
+(* An algebraic presentation of ALL using action trees. *)
+
+open FStar.Tactics
+open FStar.List.Tot
+open FStar.Universe
+
+#set-options "--print_universes --print_implicits --print_effect_args"
+
+// GM: Force a type equality by SMT
+let coerce #a #b (x:a{a == b}) : b = x
+
+let unreachable (#a:Type u#aa) () : Pure a (requires False) (ensures (fun _ -> False)) =
+  coerce #(raise_t string) #a (raise_val "whatever")
+
+type eff_label =
+  | RD
+  | WR
+  | EXN
+
+type annot = eff_label -> bool
+
+type state = int
+
+noeq
+type action : Type0 -> Type0 -> Type u#1 =
+  | Read : action unit state
+  | Write : action state unit
+  | Raise : #a:Type0 -> action exn a
+  
+noeq
+type repr0 (a:Type u#aa) : Type u#(max 1 aa) =
+  | Return : a -> repr0 a
+  | Act    : #i:_ -> #o:_ -> action i o -> i -> (o -> repr0 a) -> repr0 a
+  
+let abides_act #i #o (ann:annot) (a : action i o) : prop =
+    (Read? a ==> ann RD)
+  /\ (Write ? a ==> ann WR)
+  /\ (Raise ? a ==> ann EXN)
+
+let rec abides #a (ann:annot) (f : repr0 a) : prop =
+  begin match f with
+  | Act a i k ->
+    abides_act ann a /\ (forall o. (FStar.WellFounded.axiom1 k o; abides ann (k o)))
+  | Return _ -> True
+  end
+
+let interp (l : list eff_label) : annot =
+  fun lab -> mem lab l
+
+let rec interp_at (l1 l2 : list eff_label) (l : eff_label)
+  : Lemma (interp (l1@l2) l == (interp l1 l || interp l2 l))
+          [SMTPat (interp (l1@l2) l)]
+  = match l1 with
+    | [] -> ()
+    | _::l1 -> interp_at l1 l2 l
+    
+let sublist (l1 l2 : list eff_label) =
+  forall x. mem x l1 ==> mem x l2
+
+let sublist_refl
+  (l : list eff_label)
+  : Lemma (sublist l l)
+          [SMTPat (sublist l l)]
+  = ()
+
+let rec interp_sublist (l1 l2 : list eff_label) (l : eff_label)
+  : Lemma (requires (sublist l1 l2))
+          (ensures (interp l1 l ==> interp l2 l))
+          [SMTPat (interp l1 l); SMTPat (sublist l1 l2)]
+  = match l1 with
+    | [] -> ()
+    | _::l1 -> interp_sublist l1 l2 l
+
+let rec sublist_at
+  (l1 l2 : list eff_label)
+  : Lemma (sublist l1 (l1@l2) /\ sublist l2 (l1@l2))
+          [SMTPatOr [[SMTPat (sublist l1 (l1@l2))];
+                     [SMTPat (sublist l2 (l1@l2))]]]
+  = match l1 with
+    | [] -> ()
+    | _::l1 -> sublist_at l1 l2
+
+let rec abides_sublist #a (l1 l2 : list eff_label) (c : repr0 a)
+  : Lemma (requires (abides (interp l1) c) /\ sublist l1 l2)
+          (ensures (abides (interp l2) c))
+          [SMTPat (abides (interp l2) c); SMTPat (sublist l1 l2)]
+  = match c with
+    | Return _ -> ()
+    | Act a i k -> 
+      let sub o : Lemma (abides (interp l2) (k o)) =
+        FStar.WellFounded.axiom1 k o;
+        abides_sublist l1 l2 (k o)
+      in
+      Classical.forall_intro sub
+
+let rec abides_app #a (l1 l2 : list eff_label) (c : repr0 a)
+  : Lemma (requires (abides (interp l1) c \/ abides (interp l2) c))
+          (ensures (abides (interp (l1@l2)) c))
+          [SMTPat (abides (interp (l1@l2)) c)]
+  = // GM: Just copied the proof from above since it ought to work,
+    //     do something smarter later.
+    match c with
+    | Return _ -> ()
+    | Act a i k -> 
+      let sub o : Lemma (abides (interp (l1@l2)) (k o)) =
+        FStar.WellFounded.axiom1 k o;
+        abides_app l1 l2 (k o)
+      in
+      Classical.forall_intro sub
+
+
+type repr (a:Type u#aa)
+          (labs : list u#0 eff_label) // GM: why do I need this annot...? seems we get an ill-formed type if not
+                                      // somehow it's about `type` instead of `let`
+  : Type u#(max 1 aa)
+  =
+  r:(repr0 a){abides (interp labs) r}
+
+let ann_le (ann1 ann2 : annot) : prop =
+  forall x. ann1 x ==> ann2 x
+  
+let return (a:Type) (x:a)
+  : repr a []
+  =
+  Return x
+
+let rec bind (a b : Type)
+  (labs1 labs2 : list eff_label)
+  (c : repr a labs1)
+  (f : (x:a -> repr b labs2))
+  : Tot (repr b (labs1@labs2))
+  = match c with
+    | Return x -> f x
+    | Act a i k -> 
+      let k' o : repr b (labs1@labs2) =
+        FStar.WellFounded.axiom1 k o;
+        bind _ _ _ _ (k o) f
+      in
+      Act a i k'
+
+let subcomp (a:Type)
+  (labs1 labs2 : list eff_label)
+  (f : repr a labs1)
+  : Pure (repr a labs2)
+         (requires (sublist labs1 labs2))
+         (ensures (fun _ -> True))
+  = f
+
+let ite (p q r : Type0) = (p ==> q) /\ (~p ==> r)
+
+let if_then_else
+  (a : Type)
+  (labs1 labs2 : list eff_label)
+  (f : repr a labs1)
+  (g : repr a labs2)
+  (p : Type0)
+  : Type
+  = repr a (labs1@labs2)
+
+[@@smt_reifiable_layered_effect]
+total // need this for catch!!
+reifiable
+reflectable
+layered_effect {
+  EFF : a:Type -> list eff_label  -> Effect
+  with
+  repr         = repr;
+  return       = return;
+  bind         = bind;
+  subcomp      = subcomp;
+  if_then_else = if_then_else
+}
+
+unfold
+let pure_monotonic #a (wp : pure_wp a) : Type =
+  forall p1 p2. (forall x. p1 x ==> p2 x) ==> wp p1 ==> wp p2
+
+//unfold
+//let sp #a (wp : pure_wp a) : pure_post a =
+//  fun x -> ~ (wp (fun y -> ~(x == y)))
+
+let lift_pure_eff
+ (a:Type)
+ (wp : pure_wp a)
+ (f : unit -> PURE a wp)
+ : Pure (repr a [])
+        (requires (wp (fun _ -> True) /\ pure_monotonic wp))
+        (ensures (fun _ -> True))
+ = Return (f ())
+ 
+sub_effect PURE ~> EFF = lift_pure_eff
+
+let get () : EFF int [RD] =
+  EFF?.reflect (Act Read () Return)
+  
+let put (s:state) : EFF unit [WR] =
+  EFF?.reflect (Act Write s Return)
+
+let raise #a (e:exn) : EFF a [EXN] =
+  EFF?.reflect (Act Raise e Return)
+
+exception Failure of string
+
+let test0 (x y : int) : EFF int [RD; EXN] =
+  let z = get () in
+  if x + z > 0
+  then raise (Failure "oops")
+  else y - z
+
+let test1 (x y : int) : EFF int [EXN; RD; WR] =
+  let z = get () in
+  if x + z > 0
+  then raise (Failure "asd")
+  else (put 42; y - z)
+
+let sublist_at_self (l1 : list eff_label)
+  : Lemma (sublist (l1@l1) l1)
+          [SMTPat (l1@l1)]
+  = Classical.forall_intro (List.Tot.Properties.append_mem l1 l1)
+
+let labpoly #labs (f g : unit -> EFF int labs) : EFF int labs =
+  f () + g ()
+
+// FIXME: putting this definition inside catch causes a blowup:
+//
+// Unexpected error
+// Failure("Empty option")
+// Raised at file "stdlib.ml", line 29, characters 17-33
+// Called from file "ulib/ml/FStar_All.ml" (inlined), line 4, characters 21-24
+// Called from file "src/ocaml-output/FStar_TypeChecker_Util.ml", line 874, characters 18-65
+// Called from file "src/ocaml-output/FStar_TypeChecker_Common.ml", line 675, characters 34-38
+// Called from file "src/ocaml-output/FStar_TypeChecker_Common.ml", line 657, characters 25-33
+// Called from file "src/ocaml-output/FStar_TypeChecker_TcTerm.ml", line 2048, characters 30-68
+// Called from file "src/basic/ml/FStar_Util.ml", line 24, characters 14-18
+// ....
+let rec catch0 #a #labs (t1 : repr a (EXN::labs))
+                    (t2 : repr a labs)
+  : repr a labs
+  = match t1 with
+    | Act Raise e _ -> t2
+    | Act act i k ->
+      let k' o : repr a labs =
+        FStar.WellFounded.axiom1 k o;
+        catch0 (k o) t2
+      in
+      Act act i k'
+    | Return v -> Return v
+   | _ -> unreachable ()
+
+(* no rollback *)
+let catch #a #labs
+  (f : unit -> EFF a (EXN::labs))
+  (g : unit -> EFF a labs)
+  : EFF a labs
+=
+ EFF?.reflect begin
+   catch0 (reify (f ())) (reify (g ()))
+ end
+
+// TODO: haskell-like runST.
+// strong update with index on state type(s)?
+
+let test_catch #labs (f : unit -> EFF int [EXN;WR]) : EFF int [WR] =
+  catch f (fun () -> 42)
+
+let test_catch2 (f : unit -> EFF int [EXN;EXN;WR]) : EFF int [EXN;WR] =
+  catch f (fun () -> 42)
